SP1Clean.lean
@@ -12,11 +12,11 @@ import SP1Clean.Reader.ALUTypeReader
 import SP1Clean.Reader.CPUState
 import SP1Clean.Reader.ITypeReader
 import SP1Clean.Reader.RTypeReader
-import SP1Clean.AddiChip
+import SP1Clean.AddiChip.SailBridge
 import SP1Clean.AddChip.SailBridge
 import SP1Clean.SubChip
 import SP1Clean.SubwChip
-import SP1Clean.AddwChip
+import SP1Clean.AddwChip.SailBridge
 import SP1Clean.UTypeChip
 import SP1Clean.JalrChip
 import SP1Clean.LtChip
